Sorting/HybridSorts.v
@@ -1,0 +1,24 @@
+Add Rec LoadPath "/home/zeimer/Code/Coq".
+
+Require Import InsertionSort.
+Require Import SelectionSort.
+Require Import QuickSort.
+Require Import MergeSort2.
+
+Set Implicit Arguments.
+
+Function hqs (A : LinDec) (n : nat) (l : list A) {measure length l} : list A :=
+  if @leqb natle (length l) n
+  then insertionSort A l
+  else match l with
+      | [] => []
+      | h :: t =>
+          let (lo, hi) := bifilter (fun x : A => x <=? h) t in
+              hqs A n lo ++ h :: hqs A n hi
+  end.
+Proof.
+  intros. rewrite bifilter_spec in teq1. inversion teq1.
+    apply filter_lengthOrder.
+  intros. rewrite bifilter_spec in teq1. inversion teq1.
+    apply filter_lengthOrder.
+Defined.
