Sorting/MergeSort2.v
@@ -1,0 +1,42 @@
+Add Rec LoadPath "/home/zeimer/Code/Coq".
+
+Require Export Coq.Program.Wf.
+Require Export Recdef.
+Require Export Div2.
+
+Require Export Sort.
+Require Export ListLemmas.
+
+Set Implicit Arguments.
+
+Function merge2 (A : LinDec) (l : list A * list A)
+    {measure lenSum l} : list A :=
+let (l1, l2) := l in match l1, l2 with
+    | [], _ => l2
+    | _, [] => l1
+    | h :: t, h' :: t' =>
+        if h <=? h'
+        then h :: merge2 A (t, l2)
+        else h' :: merge2 A (l1, t')
+end.
+Proof.
+  intros. unfold lenSum. simpl. omega.
+  intros. unfold lenSum. simpl. omega.
+Defined.
+
+Function msFun2 (A : LinDec) (l : list A) {measure length l} : list A :=
+match l with
+    | [] => []
+    | [x] => [x]
+    | l' =>
+        let n := Nat.div2 (length l') in
+        let l1 := take n l' in
+        let l2 := drop n l' in
+          merge2 A (msFun2 A l1, msFun2 A l2)
+end.
+Proof.
+  intros. apply drop_length_lt. simpl. omega. inversion 1.
+  intros. apply take_length_lt. apply lt_div2. simpl. omega.
+Defined.
+
+Compute msFun2 natle testl.
