Sorting/MergeSort2Spec.v
@@ -1,0 +1,49 @@
+Add Rec LoadPath "/home/zeimer/Code/Coq".
+
+Require Import MergeSort2.
+
+Set Implicit Arguments.
+
+Theorem merge2_sorted :
+  forall (A : LinDec) (l : list A * list A),
+    sorted A (fst l) -> sorted A (snd l) -> sorted A (merge2 A l).
+Proof.
+  intros. functional induction merge2 A l; simpl in *; auto;
+  rewrite merge2_equation in *.
+    destruct t; simpl in *; dec.
+    destruct t'; simpl in *; dec.
+Qed.
+
+Theorem merge2_perm :
+  forall (A : LinDec) (l : list A * list A),
+    perm A (fst l ++ snd l) (merge2 A l).
+Proof.
+  intros. functional induction merge2 A l; simpl; auto; try clear y.
+    rewrite app_nil_r. auto.
+    eapply perm_trans.
+      rewrite app_comm_cons. apply perm_app_comm.
+      simpl. apply perm_cons. simpl in IHl0. rewrite <- IHl0.
+        apply perm_app_comm.
+Qed.
+
+Theorem msFun2_sorted :
+  forall (A : LinDec) (l : list A), sorted A (msFun2 A l).
+Proof.
+  intros. functional induction msFun2 A l; auto; clear y.
+  apply merge2_sorted; simpl; assumption.
+Qed.
+
+Theorem msFun2_perm :
+  forall (A : LinDec) (l : list A), perm A l (msFun2 A l).
+Proof.
+  intros. functional induction msFun2 A l; auto; clear y.
+  rewrite <- merge2_perm, <- (take_drop (Nat.div2 (length l))) at 1; simpl.
+  apply perm_app; assumption.
+Qed.
+
+Instance Sort_msFun2 : Sort :=
+{
+    sort := msFun2;
+    sort_sorted := msFun2_sorted;
+    sort_perm := msFun2_perm;
+}.
