Sorting/SortSpec.v
@@ -1,0 +1,37 @@
+Add Rec LoadPath "/home/zeimer/Code/Coq".
+
+Require Export Sort.
+Require Export ListLemmas.
+
+Set Implicit Arguments.
+
+(* Properties of sorting *)
+Theorem sort_nil :
+  forall (A : LinDec) (C : Sort), @sort C A [] = [].
+Proof.
+  intros. assert (perm A [] (sort [])) by (destruct C; auto).
+  red in H. simpl in H. destruct (sort []).
+    auto.
+    specialize (H c). simpl in H. dec.
+Qed.
+
+Theorem sort_cons :
+  forall (A : LinDec) (C : Sort) (h : A) (t : list A),
+    let m := min_dflt A h t in
+      @sort C A (h :: t) = m :: @sort C A (remove_once m (h :: t)).
+Proof.
+  intros. assert (sorted A (sort (h :: t))) by (destruct C; auto).
+  case_eq (sort (h :: t)); intros.
+    assert (perm A (h :: t) (sort (h :: t))) by (destruct C; auto).
+      rewrite H0 in H1. red in H1; simpl in H1. specialize (H1 h). dec.
+    rewrite H0 in H. Check sorted_cons_conv.
+      assert (wut := sorted_cons_conv A c l H).
+Abort.
+
+Theorem sort_metaspec :
+  forall (A : LinDec) (C C' : Sort) (l : list A),
+    @sort C A l = @sort C' A l.
+Proof.
+  destruct l as [| h t].
+    assert (sort [] = []).
+Abort.
