Sorting/Test.v
@@ -1,0 +1,31 @@
+Add Rec LoadPath "/home/zeimer/Code/Coq".
+
+Require Import InsertionSort.
+Require Import SelectionSort.
+Require Import QuickSort.
+Require Import MergeSort2.
+
+Require Import HybridSorts.
+
+Set Implicit Arguments.
+
+Time Eval compute in insertionSort natle testl.
+Time Eval compute in ssFun natle testl.
+Time Eval compute in qsFun natle testl.
+Time Eval compute in msFun2 natle testl.
+
+Fixpoint cycle {A : Type} (n : nat) (l : list A) : list A :=
+match n with
+    | 0 => []
+    | S n' => l ++ cycle n' l
+end.
+
+Time Compute insertionSort natle (cycle 200 testl). (* 0.304 *)
+(*Time Compute ssFun natle (cycle 200 testl).*)
+(*Time Compute qs natle (cycle 200 testl).       
+Time Compute qs2 natle (cycle 200 testl).      *)
+Time Compute hqs natle 2048 (cycle 200 testl).
+Time Compute msFun2 natle (cycle 200 testl).        (* 0.872 *)
+
+
+
